Benchmarks.lean
@@ -3,6 +3,11 @@ Copyright (c) 2024 Amazon.com, Inc. or its affiliates. All Rights Reserved.
 Released under Apache 2.0 license as described in the file LICENSE.
 Author(s): Alex Keizer
 -/
+import Benchmarks.SHA512_75
+import Benchmarks.SHA512_75_noKernel_noLint
 import Benchmarks.SHA512_150
+import Benchmarks.SHA512_150_noKernel_noLint
 import Benchmarks.SHA512_225
+import Benchmarks.SHA512_225_noKernel_noLint
 import Benchmarks.SHA512_400
+import Benchmarks.SHA512_400_noKernel_noLint
