Benchmarks/SHA512_75.lean
@@ -1,0 +1,17 @@
+/-
+Copyright (c) 2024 Amazon.com, Inc. or its affiliates. All Rights Reserved.
+Released under Apache 2.0 license as described in the file LICENSE.
+Author(s): Alex Keizer
+-/
+import Tactics.Sym
+import Benchmarks.Command
+import Benchmarks.SHA512
+
+open Benchmarks
+
+benchmark sha512_75 : SHA512Bench 75 := fun s0 _ h => by
+  intros
+  sym_n 75
+  simp only [h, bitvec_rules]
+  · exact (sorry : Aligned ..)
+  done
